src/safety/Markers.v
@@ -131,8 +131,8 @@ Lemma handle_typing_inv_for_markers : forall Γ E_tag n_beta Ts T_B T_R op_body 
     ctx_lookup_eff Γ E_tag = Some (n_α, n_beta, sig, ret) /\
     List.length Ts = n_α /\ types_wf Γ Ts /\
     ty_wf Γ T_B /\ ty_wf Γ T_R /\ Γ ⊢ₗ lt_of_ty_G Γ T_B <: lt_free /\ Γ ⊢ T_B <:: T_R /\
-    sig_β = inst_op_alpha n_α Ts n_beta sig /\
-    ret_β = inst_op_alpha n_α Ts n_beta ret /\
+    sig_β = inst_op_ty_args n_α Ts n_beta sig /\
+    ret_β = inst_op_ty_args n_α Ts n_beta ret /\
     (bind_tm sig_β
       :: bind_tm (type_fun ret_β lt_local (shift_ty n_beta 0 T_R))
       :: push_ty_vars n_beta any_at_free Γ)
